src/ocaml-output/FStar_Tactics_Interpreter.ml
@@ -657,20 +657,14 @@ let (uu___153 : unit) =
                                             uu___38 in
                                         let uu___37 =
                                           let uu___38 =
-                                            let uu___39 =
-                                              FStar_Syntax_Embeddings.e_list
-                                                FStar_Syntax_Embeddings.e_norm_step in
-                                            let uu___40 =
-                                              FStar_TypeChecker_NBETerm.e_list
-                                                FStar_TypeChecker_NBETerm.e_norm_step in
                                             FStar_Tactics_InterpFuns.mk_tac_step_1
-                                              Prims.int_zero "norm"
-                                              FStar_Tactics_Basic.norm
-                                              uu___39
+                                              Prims.int_zero "implies_intro"
+                                              FStar_Tactics_Basic.implies_intro
                                               FStar_Syntax_Embeddings.e_unit
-                                              FStar_Tactics_Basic.norm
-                                              uu___40
-                                              FStar_TypeChecker_NBETerm.e_unit in
+                                              FStar_Reflection_Embeddings.e_binder
+                                              FStar_Tactics_Basic.implies_intro
+                                              FStar_TypeChecker_NBETerm.e_unit
+                                              FStar_Reflection_NBEEmbeddings.e_binder in
                                           let uu___39 =
                                             let uu___40 =
                                               let uu___41 =
@@ -679,19 +673,14 @@ let (uu___153 : unit) =
                                               let uu___42 =
                                                 FStar_TypeChecker_NBETerm.e_list
                                                   FStar_TypeChecker_NBETerm.e_norm_step in
-                                              FStar_Tactics_InterpFuns.mk_tac_step_3
-                                                Prims.int_zero
-                                                "norm_term_env"
-                                                FStar_Tactics_Basic.norm_term_env
-                                                FStar_Reflection_Embeddings.e_env
+                                              FStar_Tactics_InterpFuns.mk_tac_step_1
+                                                Prims.int_zero "norm"
+                                                FStar_Tactics_Basic.norm
                                                 uu___41
-                                                FStar_Reflection_Embeddings.e_term
-                                                FStar_Reflection_Embeddings.e_term
-                                                FStar_Tactics_Basic.norm_term_env
-                                                FStar_Reflection_NBEEmbeddings.e_env
+                                                FStar_Syntax_Embeddings.e_unit
+                                                FStar_Tactics_Basic.norm
                                                 uu___42
-                                                FStar_Reflection_NBEEmbeddings.e_term
-                                                FStar_Reflection_NBEEmbeddings.e_term in
+                                                FStar_TypeChecker_NBETerm.e_unit in
                                             let uu___41 =
                                               let uu___42 =
                                                 let uu___43 =
@@ -700,114 +689,136 @@ let (uu___153 : unit) =
                                                 let uu___44 =
                                                   FStar_TypeChecker_NBETerm.e_list
                                                     FStar_TypeChecker_NBETerm.e_norm_step in
-                                                FStar_Tactics_InterpFuns.mk_tac_step_2
+                                                FStar_Tactics_InterpFuns.mk_tac_step_3
                                                   Prims.int_zero
-                                                  "norm_binder_type"
-                                                  FStar_Tactics_Basic.norm_binder_type
+                                                  "norm_term_env"
+                                                  FStar_Tactics_Basic.norm_term_env
+                                                  FStar_Reflection_Embeddings.e_env
                                                   uu___43
-                                                  FStar_Reflection_Embeddings.e_binder
-                                                  FStar_Syntax_Embeddings.e_unit
-                                                  FStar_Tactics_Basic.norm_binder_type
+                                                  FStar_Reflection_Embeddings.e_term
+                                                  FStar_Reflection_Embeddings.e_term
+                                                  FStar_Tactics_Basic.norm_term_env
+                                                  FStar_Reflection_NBEEmbeddings.e_env
                                                   uu___44
-                                                  FStar_Reflection_NBEEmbeddings.e_binder
-                                                  FStar_TypeChecker_NBETerm.e_unit in
+                                                  FStar_Reflection_NBEEmbeddings.e_term
+                                                  FStar_Reflection_NBEEmbeddings.e_term in
                                               let uu___43 =
                                                 let uu___44 =
+                                                  let uu___45 =
+                                                    FStar_Syntax_Embeddings.e_list
+                                                      FStar_Syntax_Embeddings.e_norm_step in
+                                                  let uu___46 =
+                                                    FStar_TypeChecker_NBETerm.e_list
+                                                      FStar_TypeChecker_NBETerm.e_norm_step in
                                                   FStar_Tactics_InterpFuns.mk_tac_step_2
                                                     Prims.int_zero
-                                                    "rename_to"
-                                                    FStar_Tactics_Basic.rename_to
+                                                    "norm_binder_type"
+                                                    FStar_Tactics_Basic.norm_binder_type
+                                                    uu___45
                                                     FStar_Reflection_Embeddings.e_binder
-                                                    FStar_Syntax_Embeddings.e_string
-                                                    FStar_Reflection_Embeddings.e_binder
-                                                    FStar_Tactics_Basic.rename_to
+                                                    FStar_Syntax_Embeddings.e_unit
+                                                    FStar_Tactics_Basic.norm_binder_type
+                                                    uu___46
                                                     FStar_Reflection_NBEEmbeddings.e_binder
-                                                    FStar_TypeChecker_NBETerm.e_string
-                                                    FStar_Reflection_NBEEmbeddings.e_binder in
+                                                    FStar_TypeChecker_NBETerm.e_unit in
                                                 let uu___45 =
                                                   let uu___46 =
-                                                    FStar_Tactics_InterpFuns.mk_tac_step_1
+                                                    FStar_Tactics_InterpFuns.mk_tac_step_2
                                                       Prims.int_zero
-                                                      "binder_retype"
-                                                      FStar_Tactics_Basic.binder_retype
+                                                      "rename_to"
+                                                      FStar_Tactics_Basic.rename_to
                                                       FStar_Reflection_Embeddings.e_binder
-                                                      FStar_Syntax_Embeddings.e_unit
-                                                      FStar_Tactics_Basic.binder_retype
+                                                      FStar_Syntax_Embeddings.e_string
+                                                      FStar_Reflection_Embeddings.e_binder
+                                                      FStar_Tactics_Basic.rename_to
                                                       FStar_Reflection_NBEEmbeddings.e_binder
-                                                      FStar_TypeChecker_NBETerm.e_unit in
+                                                      FStar_TypeChecker_NBETerm.e_string
+                                                      FStar_Reflection_NBEEmbeddings.e_binder in
                                                   let uu___47 =
                                                     let uu___48 =
                                                       FStar_Tactics_InterpFuns.mk_tac_step_1
                                                         Prims.int_zero
-                                                        "revert"
-                                                        FStar_Tactics_Basic.revert
+                                                        "binder_retype"
+                                                        FStar_Tactics_Basic.binder_retype
+                                                        FStar_Reflection_Embeddings.e_binder
                                                         FStar_Syntax_Embeddings.e_unit
-                                                        FStar_Syntax_Embeddings.e_unit
-                                                        FStar_Tactics_Basic.revert
-                                                        FStar_TypeChecker_NBETerm.e_unit
+                                                        FStar_Tactics_Basic.binder_retype
+                                                        FStar_Reflection_NBEEmbeddings.e_binder
                                                         FStar_TypeChecker_NBETerm.e_unit in
                                                     let uu___49 =
                                                       let uu___50 =
                                                         FStar_Tactics_InterpFuns.mk_tac_step_1
                                                           Prims.int_zero
-                                                          "clear_top"
-                                                          FStar_Tactics_Basic.clear_top
+                                                          "revert"
+                                                          FStar_Tactics_Basic.revert
                                                           FStar_Syntax_Embeddings.e_unit
                                                           FStar_Syntax_Embeddings.e_unit
-                                                          FStar_Tactics_Basic.clear_top
+                                                          FStar_Tactics_Basic.revert
                                                           FStar_TypeChecker_NBETerm.e_unit
                                                           FStar_TypeChecker_NBETerm.e_unit in
                                                       let uu___51 =
                                                         let uu___52 =
                                                           FStar_Tactics_InterpFuns.mk_tac_step_1
                                                             Prims.int_zero
-                                                            "clear"
-                                                            FStar_Tactics_Basic.clear
-                                                            FStar_Reflection_Embeddings.e_binder
+                                                            "clear_top"
+                                                            FStar_Tactics_Basic.clear_top
                                                             FStar_Syntax_Embeddings.e_unit
-                                                            FStar_Tactics_Basic.clear
-                                                            FStar_Reflection_NBEEmbeddings.e_binder
+                                                            FStar_Syntax_Embeddings.e_unit
+                                                            FStar_Tactics_Basic.clear_top
+                                                            FStar_TypeChecker_NBETerm.e_unit
                                                             FStar_TypeChecker_NBETerm.e_unit in
                                                         let uu___53 =
                                                           let uu___54 =
                                                             FStar_Tactics_InterpFuns.mk_tac_step_1
                                                               Prims.int_zero
-                                                              "rewrite"
-                                                              FStar_Tactics_Basic.rewrite
+                                                              "clear"
+                                                              FStar_Tactics_Basic.clear
                                                               FStar_Reflection_Embeddings.e_binder
                                                               FStar_Syntax_Embeddings.e_unit
-                                                              FStar_Tactics_Basic.rewrite
+                                                              FStar_Tactics_Basic.clear
                                                               FStar_Reflection_NBEEmbeddings.e_binder
                                                               FStar_TypeChecker_NBETerm.e_unit in
                                                           let uu___55 =
                                                             let uu___56 =
                                                               FStar_Tactics_InterpFuns.mk_tac_step_1
                                                                 Prims.int_zero
-                                                                "refine_intro"
-                                                                FStar_Tactics_Basic.refine_intro
+                                                                "rewrite"
+                                                                FStar_Tactics_Basic.rewrite
+                                                                FStar_Reflection_Embeddings.e_binder
                                                                 FStar_Syntax_Embeddings.e_unit
-                                                                FStar_Syntax_Embeddings.e_unit
-                                                                FStar_Tactics_Basic.refine_intro
-                                                                FStar_TypeChecker_NBETerm.e_unit
+                                                                FStar_Tactics_Basic.rewrite
+                                                                FStar_Reflection_NBEEmbeddings.e_binder
                                                                 FStar_TypeChecker_NBETerm.e_unit in
                                                             let uu___57 =
                                                               let uu___58 =
-                                                                FStar_Tactics_InterpFuns.mk_tac_step_3
+                                                                FStar_Tactics_InterpFuns.mk_tac_step_1
                                                                   Prims.int_zero
-                                                                  "t_exact"
-                                                                  FStar_Tactics_Basic.t_exact
-                                                                  FStar_Syntax_Embeddings.e_bool
-                                                                  FStar_Syntax_Embeddings.e_bool
-                                                                  FStar_Reflection_Embeddings.e_term
+                                                                  "refine_intro"
+                                                                  FStar_Tactics_Basic.refine_intro
                                                                   FStar_Syntax_Embeddings.e_unit
-                                                                  FStar_Tactics_Basic.t_exact
-                                                                  FStar_TypeChecker_NBETerm.e_bool
-                                                                  FStar_TypeChecker_NBETerm.e_bool
-                                                                  FStar_Reflection_NBEEmbeddings.e_term
+                                                                  FStar_Syntax_Embeddings.e_unit
+                                                                  FStar_Tactics_Basic.refine_intro
+                                                                  FStar_TypeChecker_NBETerm.e_unit
                                                                   FStar_TypeChecker_NBETerm.e_unit in
                                                               let uu___59 =
                                                                 let uu___60 =
-                                                                  FStar_Tactics_InterpFuns.mk_tac_step_4
+                                                                  FStar_Tactics_InterpFuns.mk_tac_step_3
+                                                                    Prims.int_zero
+                                                                    "t_exact"
+                                                                    FStar_Tactics_Basic.t_exact
+                                                                    FStar_Syntax_Embeddings.e_bool
+                                                                    FStar_Syntax_Embeddings.e_bool
+                                                                    FStar_Reflection_Embeddings.e_term
+                                                                    FStar_Syntax_Embeddings.e_unit
+                                                                    FStar_Tactics_Basic.t_exact
+                                                                    FStar_TypeChecker_NBETerm.e_bool
+                                                                    FStar_TypeChecker_NBETerm.e_bool
+                                                                    FStar_Reflection_NBEEmbeddings.e_term
+                                                                    FStar_TypeChecker_NBETerm.e_unit in
+                                                                let uu___61 =
+                                                                  let uu___62
+                                                                    =
+                                                                    FStar_Tactics_InterpFuns.mk_tac_step_4
                                                                     Prims.int_zero
                                                                     "t_apply"
                                                                     FStar_Tactics_Basic.t_apply
@@ -822,8 +833,9 @@ let (uu___153 : unit) =
                                                                     FStar_TypeChecker_NBETerm.e_bool
                                                                     FStar_Reflection_NBEEmbeddings.e_term
                                                                     FStar_TypeChecker_NBETerm.e_unit in
-                                                                let uu___61 =
-                                                                  let uu___62
+                                                                  let uu___63
+                                                                    =
+                                                                    let uu___64
                                                                     =
                                                                     FStar_Tactics_InterpFuns.mk_tac_step_3
                                                                     Prims.int_zero
@@ -838,9 +850,9 @@ let (uu___153 : unit) =
                                                                     FStar_TypeChecker_NBETerm.e_bool
                                                                     FStar_Reflection_NBEEmbeddings.e_term
                                                                     FStar_TypeChecker_NBETerm.e_unit in
-                                                                  let uu___63
+                                                                    let uu___65
                                                                     =
-                                                                    let uu___64
+                                                                    let uu___66
                                                                     =
                                                                     FStar_Tactics_InterpFuns.mk_tac_step_1
                                                                     Prims.int_zero
@@ -851,9 +863,9 @@ let (uu___153 : unit) =
                                                                     FStar_Tactics_Basic.set_options
                                                                     FStar_TypeChecker_NBETerm.e_string
                                                                     FStar_TypeChecker_NBETerm.e_unit in
-                                                                    let uu___65
+                                                                    let uu___67
                                                                     =
-                                                                    let uu___66
+                                                                    let uu___68
                                                                     =
                                                                     FStar_Tactics_InterpFuns.mk_tac_step_2
                                                                     Prims.int_zero
@@ -866,9 +878,9 @@ let (uu___153 : unit) =
                                                                     FStar_Reflection_NBEEmbeddings.e_env
                                                                     FStar_Reflection_NBEEmbeddings.e_term
                                                                     FStar_Reflection_NBEEmbeddings.e_comp in
-                                                                    let uu___67
+                                                                    let uu___69
                                                                     =
-                                                                    let uu___68
+                                                                    let uu___70
                                                                     =
                                                                     FStar_Tactics_InterpFuns.mk_tac_step_2
                                                                     Prims.int_zero
@@ -881,9 +893,9 @@ let (uu___153 : unit) =
                                                                     FStar_Reflection_NBEEmbeddings.e_env
                                                                     FStar_Reflection_NBEEmbeddings.e_term
                                                                     FStar_Reflection_NBEEmbeddings.e_term in
-                                                                    let uu___69
+                                                                    let uu___71
                                                                     =
-                                                                    let uu___70
+                                                                    let uu___72
                                                                     =
                                                                     FStar_Tactics_InterpFuns.mk_tac_step_1
                                                                     Prims.int_zero
@@ -894,9 +906,9 @@ let (uu___153 : unit) =
                                                                     FStar_Tactics_Basic.unshelve
                                                                     FStar_Reflection_NBEEmbeddings.e_term
                                                                     FStar_TypeChecker_NBETerm.e_unit in
-                                                                    let uu___71
+                                                                    let uu___73
                                                                     =
-                                                                    let uu___72
+                                                                    let uu___74
                                                                     =
                                                                     FStar_Tactics_InterpFuns.mk_tac_step_2
                                                                     Prims.int_one
@@ -906,19 +918,19 @@ let (uu___153 : unit) =
                                                                     FStar_Reflection_Embeddings.e_term
                                                                     FStar_Syntax_Embeddings.e_any
                                                                     (fun
-                                                                    uu___73
+                                                                    uu___75
                                                                     ->
                                                                     fun
-                                                                    uu___74
+                                                                    uu___76
                                                                     ->
                                                                     failwith
                                                                     "NBE unquote")
                                                                     FStar_TypeChecker_NBETerm.e_any
                                                                     FStar_Reflection_NBEEmbeddings.e_term
                                                                     FStar_TypeChecker_NBETerm.e_any in
-                                                                    let uu___73
+                                                                    let uu___75
                                                                     =
-                                                                    let uu___74
+                                                                    let uu___76
                                                                     =
                                                                     FStar_Tactics_InterpFuns.mk_tac_step_1
                                                                     Prims.int_zero
@@ -929,9 +941,9 @@ let (uu___153 : unit) =
                                                                     FStar_Tactics_Basic.prune
                                                                     FStar_TypeChecker_NBETerm.e_string
                                                                     FStar_TypeChecker_NBETerm.e_unit in
-                                                                    let uu___75
+                                                                    let uu___77
                                                                     =
-                                                                    let uu___76
+                                                                    let uu___78
                                                                     =
                                                                     FStar_Tactics_InterpFuns.mk_tac_step_1
                                                                     Prims.int_zero
@@ -942,9 +954,9 @@ let (uu___153 : unit) =
                                                                     FStar_Tactics_Basic.addns
                                                                     FStar_TypeChecker_NBETerm.e_string
                                                                     FStar_TypeChecker_NBETerm.e_unit in
-                                                                    let uu___77
+                                                                    let uu___79
                                                                     =
-                                                                    let uu___78
+                                                                    let uu___80
                                                                     =
                                                                     FStar_Tactics_InterpFuns.mk_tac_step_1
                                                                     Prims.int_zero
@@ -955,9 +967,9 @@ let (uu___153 : unit) =
                                                                     FStar_Tactics_Basic.print
                                                                     FStar_TypeChecker_NBETerm.e_string
                                                                     FStar_TypeChecker_NBETerm.e_unit in
-                                                                    let uu___79
+                                                                    let uu___81
                                                                     =
-                                                                    let uu___80
+                                                                    let uu___82
                                                                     =
                                                                     FStar_Tactics_InterpFuns.mk_tac_step_1
                                                                     Prims.int_zero
@@ -968,9 +980,9 @@ let (uu___153 : unit) =
                                                                     FStar_Tactics_Basic.debugging
                                                                     FStar_TypeChecker_NBETerm.e_unit
                                                                     FStar_TypeChecker_NBETerm.e_bool in
-                                                                    let uu___81
+                                                                    let uu___83
                                                                     =
-                                                                    let uu___82
+                                                                    let uu___84
                                                                     =
                                                                     FStar_Tactics_InterpFuns.mk_tac_step_1
                                                                     Prims.int_zero
@@ -981,9 +993,9 @@ let (uu___153 : unit) =
                                                                     FStar_Tactics_Basic.dump
                                                                     FStar_TypeChecker_NBETerm.e_string
                                                                     FStar_TypeChecker_NBETerm.e_unit in
-                                                                    let uu___83
+                                                                    let uu___85
                                                                     =
-                                                                    let uu___84
+                                                                    let uu___86
                                                                     =
                                                                     FStar_Tactics_InterpFuns.mk_tac_step_2
                                                                     Prims.int_zero
@@ -996,9 +1008,9 @@ let (uu___153 : unit) =
                                                                     FStar_TypeChecker_NBETerm.e_bool
                                                                     FStar_TypeChecker_NBETerm.e_string
                                                                     FStar_TypeChecker_NBETerm.e_unit in
-                                                                    let uu___85
+                                                                    let uu___87
                                                                     =
-                                                                    let uu___86
+                                                                    let uu___88
                                                                     =
                                                                     FStar_Tactics_InterpFuns.mk_tac_step_2
                                                                     Prims.int_zero
@@ -1011,35 +1023,35 @@ let (uu___153 : unit) =
                                                                     FStar_Tactics_Embedding.e_goal_nbe
                                                                     FStar_TypeChecker_NBETerm.e_string
                                                                     FStar_TypeChecker_NBETerm.e_unit in
-                                                                    let uu___87
-                                                                    =
-                                                                    let uu___88
-                                                                    =
                                                                     let uu___89
                                                                     =
                                                                     let uu___90
+                                                                    =
+                                                                    let uu___91
+                                                                    =
+                                                                    let uu___92
                                                                     =
                                                                     FStar_Syntax_Embeddings.e_tuple2
                                                                     FStar_Syntax_Embeddings.e_bool
                                                                     FStar_Tactics_Embedding.e_ctrl_flag in
                                                                     e_tactic_1
                                                                     FStar_Reflection_Embeddings.e_term
-                                                                    uu___90 in
-                                                                    let uu___90
+                                                                    uu___92 in
+                                                                    let uu___92
                                                                     =
                                                                     e_tactic_thunk
                                                                     FStar_Syntax_Embeddings.e_unit in
-                                                                    let uu___91
+                                                                    let uu___93
                                                                     =
-                                                                    let uu___92
+                                                                    let uu___94
                                                                     =
                                                                     FStar_TypeChecker_NBETerm.e_tuple2
                                                                     FStar_TypeChecker_NBETerm.e_bool
                                                                     FStar_Tactics_Embedding.e_ctrl_flag_nbe in
                                                                     e_tactic_nbe_1
                                                                     FStar_Reflection_NBEEmbeddings.e_term
-                                                                    uu___92 in
-                                                                    let uu___92
+                                                                    uu___94 in
+                                                                    let uu___94
                                                                     =
                                                                     e_tactic_nbe_thunk
                                                                     FStar_TypeChecker_NBETerm.e_unit in
@@ -1048,17 +1060,17 @@ let (uu___153 : unit) =
                                                                     "ctrl_rewrite"
                                                                     FStar_Tactics_CtrlRewrite.ctrl_rewrite
                                                                     FStar_Tactics_Embedding.e_direction
-                                                                    uu___89
-                                                                    uu___90
+                                                                    uu___91
+                                                                    uu___92
                                                                     FStar_Syntax_Embeddings.e_unit
                                                                     FStar_Tactics_CtrlRewrite.ctrl_rewrite
                                                                     FStar_Tactics_Embedding.e_direction_nbe
-                                                                    uu___91
-                                                                    uu___92
+                                                                    uu___93
+                                                                    uu___94
                                                                     FStar_TypeChecker_NBETerm.e_unit in
-                                                                    let uu___89
+                                                                    let uu___91
                                                                     =
-                                                                    let uu___90
+                                                                    let uu___92
                                                                     =
                                                                     FStar_Tactics_InterpFuns.mk_tac_step_1
                                                                     Prims.int_zero
@@ -1069,9 +1081,9 @@ let (uu___153 : unit) =
                                                                     FStar_Tactics_Basic.t_trefl
                                                                     FStar_TypeChecker_NBETerm.e_bool
                                                                     FStar_TypeChecker_NBETerm.e_unit in
-                                                                    let uu___91
+                                                                    let uu___93
                                                                     =
-                                                                    let uu___92
+                                                                    let uu___94
                                                                     =
                                                                     FStar_Tactics_InterpFuns.mk_tac_step_1
                                                                     Prims.int_zero
@@ -1082,9 +1094,9 @@ let (uu___153 : unit) =
                                                                     FStar_Tactics_Basic.dup
                                                                     FStar_TypeChecker_NBETerm.e_unit
                                                                     FStar_TypeChecker_NBETerm.e_unit in
-                                                                    let uu___93
+                                                                    let uu___95
                                                                     =
-                                                                    let uu___94
+                                                                    let uu___96
                                                                     =
                                                                     FStar_Tactics_InterpFuns.mk_tac_step_1
                                                                     Prims.int_zero
@@ -1095,9 +1107,9 @@ let (uu___153 : unit) =
                                                                     FStar_Tactics_Basic.tadmit_t
                                                                     FStar_Reflection_NBEEmbeddings.e_term
                                                                     FStar_TypeChecker_NBETerm.e_unit in
-                                                                    let uu___95
+                                                                    let uu___97
                                                                     =
-                                                                    let uu___96
+                                                                    let uu___98
                                                                     =
                                                                     FStar_Tactics_InterpFuns.mk_tac_step_1
                                                                     Prims.int_zero
@@ -1108,40 +1120,40 @@ let (uu___153 : unit) =
                                                                     FStar_Tactics_Basic.join
                                                                     FStar_TypeChecker_NBETerm.e_unit
                                                                     FStar_TypeChecker_NBETerm.e_unit in
-                                                                    let uu___97
-                                                                    =
-                                                                    let uu___98
-                                                                    =
                                                                     let uu___99
                                                                     =
                                                                     let uu___100
+                                                                    =
+                                                                    let uu___101
+                                                                    =
+                                                                    let uu___102
                                                                     =
                                                                     FStar_Syntax_Embeddings.e_tuple2
                                                                     FStar_Reflection_Embeddings.e_fv
                                                                     FStar_Syntax_Embeddings.e_int in
                                                                     FStar_Syntax_Embeddings.e_list
-                                                                    uu___100 in
-                                                                    let uu___100
+                                                                    uu___102 in
+                                                                    let uu___102
                                                                     =
-                                                                    let uu___101
+                                                                    let uu___103
                                                                     =
                                                                     FStar_TypeChecker_NBETerm.e_tuple2
                                                                     FStar_Reflection_NBEEmbeddings.e_fv
                                                                     FStar_TypeChecker_NBETerm.e_int in
                                                                     FStar_TypeChecker_NBETerm.e_list
-                                                                    uu___101 in
+                                                                    uu___103 in
                                                                     FStar_Tactics_InterpFuns.mk_tac_step_1
                                                                     Prims.int_zero
                                                                     "t_destruct"
                                                                     FStar_Tactics_Basic.t_destruct
                                                                     FStar_Reflection_Embeddings.e_term
-                                                                    uu___99
+                                                                    uu___101
                                                                     FStar_Tactics_Basic.t_destruct
                                                                     FStar_Reflection_NBEEmbeddings.e_term
-                                                                    uu___100 in
-                                                                    let uu___99
+                                                                    uu___102 in
+                                                                    let uu___101
                                                                     =
-                                                                    let uu___100
+                                                                    let uu___102
                                                                     =
                                                                     FStar_Tactics_InterpFuns.mk_tac_step_1
                                                                     Prims.int_zero
@@ -1152,9 +1164,9 @@ let (uu___153 : unit) =
                                                                     FStar_Tactics_Basic.top_env
                                                                     FStar_TypeChecker_NBETerm.e_unit
                                                                     FStar_Reflection_NBEEmbeddings.e_env in
-                                                                    let uu___101
+                                                                    let uu___103
                                                                     =
-                                                                    let uu___102
+                                                                    let uu___104
                                                                     =
                                                                     FStar_Tactics_InterpFuns.mk_tac_step_1
                                                                     Prims.int_zero
@@ -1165,9 +1177,9 @@ let (uu___153 : unit) =
                                                                     FStar_Tactics_Basic.inspect
                                                                     FStar_Reflection_NBEEmbeddings.e_term
                                                                     FStar_Reflection_NBEEmbeddings.e_term_view in
-                                                                    let uu___103
+                                                                    let uu___105
                                                                     =
-                                                                    let uu___104
+                                                                    let uu___106
                                                                     =
                                                                     FStar_Tactics_InterpFuns.mk_tac_step_1
                                                                     Prims.int_zero
@@ -1178,9 +1190,9 @@ let (uu___153 : unit) =
                                                                     FStar_Tactics_Basic.pack
                                                                     FStar_Reflection_NBEEmbeddings.e_term_view
                                                                     FStar_Reflection_NBEEmbeddings.e_term in
-                                                                    let uu___105
+                                                                    let uu___107
                                                                     =
-                                                                    let uu___106
+                                                                    let uu___108
                                                                     =
                                                                     FStar_Tactics_InterpFuns.mk_tac_step_1
                                                                     Prims.int_zero
@@ -1191,9 +1203,9 @@ let (uu___153 : unit) =
                                                                     FStar_Tactics_Basic.pack_curried
                                                                     FStar_Reflection_NBEEmbeddings.e_term_view
                                                                     FStar_Reflection_NBEEmbeddings.e_term in
-                                                                    let uu___107
+                                                                    let uu___109
                                                                     =
-                                                                    let uu___108
+                                                                    let uu___110
                                                                     =
                                                                     FStar_Tactics_InterpFuns.mk_tac_step_1
                                                                     Prims.int_zero
@@ -1204,9 +1216,9 @@ let (uu___153 : unit) =
                                                                     FStar_Tactics_Basic.fresh
                                                                     FStar_TypeChecker_NBETerm.e_unit
                                                                     FStar_TypeChecker_NBETerm.e_int in
-                                                                    let uu___109
+                                                                    let uu___111
                                                                     =
-                                                                    let uu___110
+                                                                    let uu___112
                                                                     =
                                                                     FStar_Tactics_InterpFuns.mk_tac_step_1
                                                                     Prims.int_zero
@@ -1217,15 +1229,15 @@ let (uu___153 : unit) =
                                                                     FStar_Tactics_Basic.curms
                                                                     FStar_TypeChecker_NBETerm.e_unit
                                                                     FStar_TypeChecker_NBETerm.e_int in
-                                                                    let uu___111
-                                                                    =
-                                                                    let uu___112
-                                                                    =
                                                                     let uu___113
+                                                                    =
+                                                                    let uu___114
+                                                                    =
+                                                                    let uu___115
                                                                     =
                                                                     FStar_Syntax_Embeddings.e_option
                                                                     FStar_Reflection_Embeddings.e_term in
-                                                                    let uu___114
+                                                                    let uu___116
                                                                     =
                                                                     FStar_TypeChecker_NBETerm.e_option
                                                                     FStar_Reflection_NBEEmbeddings.e_term in
@@ -1234,15 +1246,15 @@ let (uu___153 : unit) =
                                                                     "uvar_env"
                                                                     FStar_Tactics_Basic.uvar_env
                                                                     FStar_Reflection_Embeddings.e_env
-                                                                    uu___113
+                                                                    uu___115
                                                                     FStar_Reflection_Embeddings.e_term
                                                                     FStar_Tactics_Basic.uvar_env
                                                                     FStar_Reflection_NBEEmbeddings.e_env
-                                                                    uu___114
+                                                                    uu___116
                                                                     FStar_Reflection_NBEEmbeddings.e_term in
-                                                                    let uu___113
+                                                                    let uu___115
                                                                     =
-                                                                    let uu___114
+                                                                    let uu___116
                                                                     =
                                                                     FStar_Tactics_InterpFuns.mk_tac_step_1
                                                                     Prims.int_zero
@@ -1253,9 +1265,9 @@ let (uu___153 : unit) =
                                                                     FStar_Tactics_Basic.fresh_universe_uvar
                                                                     FStar_TypeChecker_NBETerm.e_unit
                                                                     FStar_Reflection_NBEEmbeddings.e_term in
-                                                                    let uu___115
+                                                                    let uu___117
                                                                     =
-                                                                    let uu___116
+                                                                    let uu___118
                                                                     =
                                                                     FStar_Tactics_InterpFuns.mk_tac_step_3
                                                                     Prims.int_zero
@@ -1270,9 +1282,9 @@ let (uu___153 : unit) =
                                                                     FStar_Reflection_NBEEmbeddings.e_term
                                                                     FStar_Reflection_NBEEmbeddings.e_term
                                                                     FStar_TypeChecker_NBETerm.e_bool in
-                                                                    let uu___117
+                                                                    let uu___119
                                                                     =
-                                                                    let uu___118
+                                                                    let uu___120
                                                                     =
                                                                     FStar_Tactics_InterpFuns.mk_tac_step_3
                                                                     Prims.int_zero
@@ -1287,9 +1299,9 @@ let (uu___153 : unit) =
                                                                     FStar_Reflection_NBEEmbeddings.e_term
                                                                     FStar_Reflection_NBEEmbeddings.e_term
                                                                     FStar_TypeChecker_NBETerm.e_bool in
-                                                                    let uu___119
+                                                                    let uu___121
                                                                     =
-                                                                    let uu___120
+                                                                    let uu___122
                                                                     =
                                                                     FStar_Tactics_InterpFuns.mk_tac_step_3
                                                                     Prims.int_zero
@@ -1304,15 +1316,15 @@ let (uu___153 : unit) =
                                                                     FStar_Reflection_NBEEmbeddings.e_term
                                                                     FStar_Reflection_NBEEmbeddings.e_term
                                                                     FStar_TypeChecker_NBETerm.e_bool in
-                                                                    let uu___121
-                                                                    =
-                                                                    let uu___122
-                                                                    =
                                                                     let uu___123
+                                                                    =
+                                                                    let uu___124
+                                                                    =
+                                                                    let uu___125
                                                                     =
                                                                     FStar_Syntax_Embeddings.e_list
                                                                     FStar_Syntax_Embeddings.e_string in
-                                                                    let uu___124
+                                                                    let uu___126
                                                                     =
                                                                     FStar_TypeChecker_NBETerm.e_list
                                                                     FStar_TypeChecker_NBETerm.e_string in
@@ -1321,17 +1333,17 @@ let (uu___153 : unit) =
                                                                     "launch_process"
                                                                     FStar_Tactics_Basic.launch_process
                                                                     FStar_Syntax_Embeddings.e_string
-                                                                    uu___123
+                                                                    uu___125
                                                                     FStar_Syntax_Embeddings.e_string
                                                                     FStar_Syntax_Embeddings.e_string
                                                                     FStar_Tactics_Basic.launch_process
                                                                     FStar_TypeChecker_NBETerm.e_string
-                                                                    uu___124
+                                                                    uu___126
                                                                     FStar_TypeChecker_NBETerm.e_string
                                                                     FStar_TypeChecker_NBETerm.e_string in
-                                                                    let uu___123
+                                                                    let uu___125
                                                                     =
-                                                                    let uu___124
+                                                                    let uu___126
                                                                     =
                                                                     FStar_Tactics_InterpFuns.mk_tac_step_2
                                                                     Prims.int_zero
@@ -1344,9 +1356,9 @@ let (uu___153 : unit) =
                                                                     FStar_TypeChecker_NBETerm.e_string
                                                                     FStar_Reflection_NBEEmbeddings.e_term
                                                                     FStar_Reflection_NBEEmbeddings.e_bv in
-                                                                    let uu___125
+                                                                    let uu___127
                                                                     =
-                                                                    let uu___126
+                                                                    let uu___128
                                                                     =
                                                                     FStar_Tactics_InterpFuns.mk_tac_step_1
                                                                     Prims.int_zero
@@ -1357,9 +1369,9 @@ let (uu___153 : unit) =
                                                                     FStar_Tactics_Basic.change
                                                                     FStar_Reflection_NBEEmbeddings.e_term
                                                                     FStar_TypeChecker_NBETerm.e_unit in
-                                                                    let uu___127
+                                                                    let uu___129
                                                                     =
-                                                                    let uu___128
+                                                                    let uu___130
                                                                     =
                                                                     FStar_Tactics_InterpFuns.mk_tac_step_1
                                                                     Prims.int_zero
@@ -1370,9 +1382,9 @@ let (uu___153 : unit) =
                                                                     FStar_Tactics_Basic.get_guard_policy
                                                                     FStar_TypeChecker_NBETerm.e_unit
                                                                     FStar_Tactics_Embedding.e_guard_policy_nbe in
-                                                                    let uu___129
+                                                                    let uu___131
                                                                     =
-                                                                    let uu___130
+                                                                    let uu___132
                                                                     =
                                                                     FStar_Tactics_InterpFuns.mk_tac_step_1
                                                                     Prims.int_zero
@@ -1383,9 +1395,9 @@ let (uu___153 : unit) =
                                                                     FStar_Tactics_Basic.set_guard_policy
                                                                     FStar_Tactics_Embedding.e_guard_policy_nbe
                                                                     FStar_TypeChecker_NBETerm.e_unit in
-                                                                    let uu___131
+                                                                    let uu___133
                                                                     =
-                                                                    let uu___132
+                                                                    let uu___134
                                                                     =
                                                                     FStar_Tactics_InterpFuns.mk_tac_step_1
                                                                     Prims.int_zero
@@ -1396,9 +1408,9 @@ let (uu___153 : unit) =
                                                                     FStar_Tactics_Basic.lax_on
                                                                     FStar_TypeChecker_NBETerm.e_unit
                                                                     FStar_TypeChecker_NBETerm.e_bool in
-                                                                    let uu___133
+                                                                    let uu___135
                                                                     =
-                                                                    let uu___134
+                                                                    let uu___136
                                                                     =
                                                                     FStar_Tactics_InterpFuns.mk_tac_step_2
                                                                     Prims.int_one
@@ -1408,19 +1420,19 @@ let (uu___153 : unit) =
                                                                     FStar_Syntax_Embeddings.e_string
                                                                     FStar_Syntax_Embeddings.e_any
                                                                     (fun
-                                                                    uu___135
+                                                                    uu___137
                                                                     ->
                                                                     fun
-                                                                    uu___136
+                                                                    uu___138
                                                                     ->
                                                                     FStar_Tactics_Monad.fail
                                                                     "sorry, `lget` does not work in NBE")
                                                                     FStar_TypeChecker_NBETerm.e_any
                                                                     FStar_TypeChecker_NBETerm.e_string
                                                                     FStar_TypeChecker_NBETerm.e_any in
-                                                                    let uu___135
+                                                                    let uu___137
                                                                     =
-                                                                    let uu___136
+                                                                    let uu___138
                                                                     =
                                                                     FStar_Tactics_InterpFuns.mk_tac_step_3
                                                                     Prims.int_one
@@ -1431,13 +1443,13 @@ let (uu___153 : unit) =
                                                                     FStar_Syntax_Embeddings.e_any
                                                                     FStar_Syntax_Embeddings.e_unit
                                                                     (fun
-                                                                    uu___137
-                                                                    ->
-                                                                    fun
-                                                                    uu___138
-                                                                    ->
-                                                                    fun
                                                                     uu___139
+                                                                    ->
+                                                                    fun
+                                                                    uu___140
+                                                                    ->
+                                                                    fun
+                                                                    uu___141
                                                                     ->
                                                                     FStar_Tactics_Monad.fail
                                                                     "sorry, `lset` does not work in NBE")
@@ -1445,9 +1457,9 @@ let (uu___153 : unit) =
                                                                     FStar_TypeChecker_NBETerm.e_string
                                                                     FStar_TypeChecker_NBETerm.e_any
                                                                     FStar_TypeChecker_NBETerm.e_unit in
-                                                                    let uu___137
+                                                                    let uu___139
                                                                     =
-                                                                    let uu___138
+                                                                    let uu___140
                                                                     =
                                                                     FStar_Tactics_InterpFuns.mk_tac_step_1
                                                                     Prims.int_one
@@ -1458,9 +1470,9 @@ let (uu___153 : unit) =
                                                                     FStar_Tactics_Basic.set_urgency
                                                                     FStar_TypeChecker_NBETerm.e_int
                                                                     FStar_TypeChecker_NBETerm.e_unit in
-                                                                    let uu___139
+                                                                    let uu___141
                                                                     =
-                                                                    let uu___140
+                                                                    let uu___142
                                                                     =
                                                                     FStar_Tactics_InterpFuns.mk_tac_step_1
                                                                     Prims.int_one
@@ -1471,9 +1483,9 @@ let (uu___153 : unit) =
                                                                     FStar_Tactics_Basic.t_commute_applied_match
                                                                     FStar_TypeChecker_NBETerm.e_unit
                                                                     FStar_TypeChecker_NBETerm.e_unit in
-                                                                    let uu___141
+                                                                    let uu___143
                                                                     =
-                                                                    let uu___142
+                                                                    let uu___144
                                                                     =
                                                                     FStar_Tactics_InterpFuns.mk_tac_step_1
                                                                     Prims.int_zero
@@ -1484,9 +1496,9 @@ let (uu___153 : unit) =
                                                                     FStar_Tactics_Basic.gather_explicit_guards_for_resolved_goals
                                                                     FStar_TypeChecker_NBETerm.e_unit
                                                                     FStar_TypeChecker_NBETerm.e_unit in
-                                                                    let uu___143
+                                                                    let uu___145
                                                                     =
-                                                                    let uu___144
+                                                                    let uu___146
                                                                     =
                                                                     FStar_Tactics_InterpFuns.mk_tac_step_2
                                                                     Prims.int_zero
@@ -1499,16 +1511,16 @@ let (uu___153 : unit) =
                                                                     FStar_Reflection_NBEEmbeddings.e_env
                                                                     FStar_TypeChecker_NBETerm.e_string
                                                                     FStar_Reflection_NBEEmbeddings.e_term in
-                                                                    let uu___145
-                                                                    =
-                                                                    let uu___146
-                                                                    =
                                                                     let uu___147
+                                                                    =
+                                                                    let uu___148
+                                                                    =
+                                                                    let uu___149
                                                                     =
                                                                     FStar_Syntax_Embeddings.e_tuple2
                                                                     FStar_Reflection_Embeddings.e_env
                                                                     FStar_Reflection_Embeddings.e_bv in
-                                                                    let uu___148
+                                                                    let uu___150
                                                                     =
                                                                     FStar_TypeChecker_NBETerm.e_tuple2
                                                                     FStar_Reflection_NBEEmbeddings.e_env
@@ -1519,14 +1531,14 @@ let (uu___153 : unit) =
                                                                     FStar_Tactics_Basic.push_bv_dsenv
                                                                     FStar_Reflection_Embeddings.e_env
                                                                     FStar_Syntax_Embeddings.e_string
-                                                                    uu___147
+                                                                    uu___149
                                                                     FStar_Tactics_Basic.push_bv_dsenv
                                                                     FStar_Reflection_NBEEmbeddings.e_env
                                                                     FStar_TypeChecker_NBETerm.e_string
-                                                                    uu___148 in
-                                                                    let uu___147
+                                                                    uu___150 in
+                                                                    let uu___149
                                                                     =
-                                                                    let uu___148
+                                                                    let uu___150
                                                                     =
                                                                     FStar_Tactics_InterpFuns.mk_tac_step_1
                                                                     Prims.int_zero
@@ -1537,9 +1549,9 @@ let (uu___153 : unit) =
                                                                     FStar_Tactics_Basic.term_to_string
                                                                     FStar_Reflection_NBEEmbeddings.e_term
                                                                     FStar_TypeChecker_NBETerm.e_string in
-                                                                    let uu___149
+                                                                    let uu___151
                                                                     =
-                                                                    let uu___150
+                                                                    let uu___152
                                                                     =
                                                                     FStar_Tactics_InterpFuns.mk_tac_step_1
                                                                     Prims.int_zero
@@ -1550,9 +1562,9 @@ let (uu___153 : unit) =
                                                                     FStar_Tactics_Basic.comp_to_string
                                                                     FStar_Reflection_NBEEmbeddings.e_comp
                                                                     FStar_TypeChecker_NBETerm.e_string in
-                                                                    let uu___151
+                                                                    let uu___154
                                                                     =
-                                                                    let uu___152
+                                                                    let uu___155
                                                                     =
                                                                     FStar_Tactics_InterpFuns.mk_tac_step_2
                                                                     Prims.int_zero
@@ -1565,15 +1577,15 @@ let (uu___153 : unit) =
                                                                     FStar_Reflection_NBEEmbeddings.e_term
                                                                     FStar_Reflection_NBEEmbeddings.e_term
                                                                     FStar_TypeChecker_NBETerm.e_bool in
-                                                                    let uu___154
-                                                                    =
-                                                                    let uu___155
-                                                                    =
                                                                     let uu___156
+                                                                    =
+                                                                    let uu___157
+                                                                    =
+                                                                    let uu___158
                                                                     =
                                                                     e_tactic_thunk
                                                                     FStar_Syntax_Embeddings.e_any in
-                                                                    let uu___157
+                                                                    let uu___159
                                                                     =
                                                                     e_tactic_nbe_thunk
                                                                     FStar_TypeChecker_NBETerm.e_any in
@@ -1581,22 +1593,25 @@ let (uu___153 : unit) =
                                                                     Prims.int_one
                                                                     "with_compat_pre_core"
                                                                     (fun
-                                                                    uu___158
+                                                                    uu___160
                                                                     ->
                                                                     FStar_Tactics_Basic.with_compat_pre_core)
                                                                     FStar_Syntax_Embeddings.e_any
                                                                     FStar_Syntax_Embeddings.e_int
-                                                                    uu___156
+                                                                    uu___158
                                                                     FStar_Syntax_Embeddings.e_any
                                                                     (fun
-                                                                    uu___158
+                                                                    uu___160
                                                                     ->
                                                                     FStar_Tactics_Basic.with_compat_pre_core)
                                                                     FStar_TypeChecker_NBETerm.e_any
                                                                     FStar_TypeChecker_NBETerm.e_int
-                                                                    uu___157
+                                                                    uu___159
                                                                     FStar_TypeChecker_NBETerm.e_any in
-                                                                    [uu___155] in
+                                                                    [uu___157] in
+                                                                    uu___155
+                                                                    ::
+                                                                    uu___156 in
                                                                     uu___152
                                                                     ::
                                                                     uu___154 in
